mailbox/acq_rel_SW.v
@@ -128,11 +128,11 @@ Program Definition load_acq_spec := TYPE LA_type
   WITH l : val, s : _, st_ord : _ -> _ -> Prop, T : ((_ -> Z -> mpred) * (_ -> Z -> mpred)),
        P : mpred, II : Z -> mpred, lI : list Z, P' : mpred, Q : _ -> Z -> mpred
   PRE [ 1%positive OF tptr tint ]
-   PROP (view_shift (fold_right sepcon emp (map (fun p => |>II p) lI) * P)
+   PROP (view_shift (fold_right sepcon emp (map II lI) * P)
                     (protocol_R l s st_ord T * P');
          forall s' v, st_ord s s' -> repable_signed v ->
            view_shift (fst T s' v * protocol_R l s' st_ord T * P')%logic
-           (fold_right sepcon emp (map (fun p => |>II p) lI) * Q s' v))
+           (fold_right sepcon emp (map II lI) * Q s' v))
    LOCAL (temp 1%positive l)
    SEP (fold_right sepcon emp (map (fun p => invariant (II p)) lI); P)
   POST [ tint ]
@@ -150,7 +150,7 @@ Proof.
       setoid_rewrite view_shift_super_non_expansive at 2; do 2 apply f_equal; f_equal.
       * rewrite !approx_sepcon, !approx_sepcon_list', approx_idem.
         erewrite !map_map, map_ext; eauto.
-        intro; simpl; rewrite nonexpansive_super_non_expansive by (apply later_nonexpansive); auto.
+        intro; simpl; rewrite approx_idem; auto.
       * unfold protocol_R; rewrite !approx_sepcon, approx_idem, protocol_piece_super_non_expansive; auto.
     + rewrite !prop_forall, !(approx_allp _ _ _ s); f_equal; extensionality s'.
       rewrite !prop_forall, !(approx_allp _ _ _ 0); f_equal; extensionality v'.
@@ -160,7 +160,7 @@ Proof.
       setoid_rewrite view_shift_super_non_expansive at 2.
       unfold protocol_R; rewrite !approx_sepcon, !approx_sepcon_list', protocol_piece_super_non_expansive, !approx_idem.
       erewrite !map_map, map_ext; eauto.
-      intro; simpl; rewrite nonexpansive_super_non_expansive by (apply later_nonexpansive); auto.
+      intro; simpl; rewrite approx_idem; auto.
   - unfold LOCALx; simpl; rewrite !approx_andp; apply f_equal.
     unfold SEPx; simpl; rewrite !sepcon_emp, !approx_sepcon, !approx_idem, !approx_sepcon_list'.
     erewrite !map_map, map_ext; eauto.
@@ -189,11 +189,11 @@ Program Definition store_rel_spec := TYPE SR_type
        P : mpred, II : Z -> mpred, lI : list Z, P' : mpred, Q : mpred
   PRE [ 1%positive OF tptr tint, 2%positive OF tint ]
    PROP (repable_signed v;
-         view_shift (fold_right sepcon emp (map (fun p => |>II p) lI) * P)
+         view_shift (fold_right sepcon emp (map II lI) * P)
                     (protocol_W l s st_ord T * P');
          forall v0, repable_signed v0 ->
            view_shift (snd T s v0 * protocol_W l s'' st_ord T * P')%logic
-                      (snd T s'' v * fold_right sepcon emp (map (fun p => |>II p) lI) * Q)%logic; st_ord s s'')
+                      (snd T s'' v * fold_right sepcon emp (map II lI) * Q)%logic; st_ord s s'')
    LOCAL (temp 1%positive l; temp 2%positive (vint v))
    SEP (fold_right sepcon emp (map (fun p => invariant (II p)) lI); P)
   POST [ tvoid ]
@@ -210,7 +210,7 @@ Proof.
       setoid_rewrite view_shift_super_non_expansive at 2; do 2 apply f_equal; f_equal.
       * rewrite !approx_sepcon, !approx_sepcon_list', approx_idem.
         erewrite !map_map, map_ext; eauto.
-        intro; simpl; rewrite nonexpansive_super_non_expansive by (apply later_nonexpansive); auto.
+        intro; simpl; rewrite approx_idem; auto.
       * unfold protocol_W; rewrite !approx_sepcon, approx_idem, protocol_piece_super_non_expansive; auto.
     + rewrite !prop_forall, !(approx_allp _ _ _ 0); f_equal; extensionality v'.
       rewrite !prop_impl; setoid_rewrite approx_imp; do 2 apply f_equal.
@@ -218,7 +218,7 @@ Proof.
       setoid_rewrite view_shift_super_non_expansive at 2.
       unfold protocol_W; rewrite !sepcon_assoc, !approx_sepcon, !approx_sepcon_list', protocol_piece_super_non_expansive, !approx_idem.
       erewrite !map_map, map_ext; eauto.
-      intro; simpl; rewrite nonexpansive_super_non_expansive by (apply later_nonexpansive); auto.
+      intro; simpl; rewrite approx_idem; auto.
   - unfold LOCALx; simpl; rewrite !approx_andp; apply f_equal.
     unfold SEPx; simpl; rewrite !sepcon_emp, !approx_sepcon, !approx_idem, !approx_sepcon_list'.
     erewrite !map_map, map_ext; eauto.
